More examples.

tests/Add.bpl
@@ -10,13 +10,16 @@ type State;
 var M: MType;
 var C: CType;
 var R: CType;
-var C#init: CType;
+var L: CType;
 var St: [Actor]State;
+const Base#L: int;
+axiom 1 <= Base#L;
 
 const unique this#: Actor;
-
 type List a = [int]a;
 var AT#intlst: List int;
+
+function AT#Min(x:int, y: int): int { if x <= y then x else y }
 
 
 // ---------------------------------------------------------------
@@ -26,8 +29,9 @@ var AT#intlst: List int;
 procedure Add#anon$0#0()
   modifies C, R, M, St;
 {
-  var IV#in1#i: int;
-  var IV#in2#j: int;
+  var IV#in1#0: int;
+  var IV#in2#0: int;
+  assume true;
   assume true;
 }
 procedure Net#init#1()
@@ -48,43 +52,44 @@ procedure Net#anon$1#entry#2()
   modifies C, R, M, St;
 {
   var ActionPH#y: int;
-  assume C#init[Net#a] == 1;
-  assume C#init[Net#b] == 1;
-  assume C#init[Net#c] == 0;
+  assume L[Net#a] == (1 * Base#L);
+  assume L[Net#b] == (1 * Base#L);
   assume R[Net#a] == 0;
+  assume C[Net#a] == 0;
   assume R[Net#b] == 0;
+  assume C[Net#b] == 0;
   assume R[Net#c] == 0;
-  assume C#init == C;
-  assert {:msg "  Channel invariant might not hold on action entry (generated #0)"} 0 <= R[Net#a];
-  assert {:msg "  Channel invariant might not hold on action entry (generated #1)"} 0 <= C[Net#a];
-  assert {:msg "  Channel invariant might not hold on action entry (generated #2)"} (R[Net#a] + C[Net#a]) == C#init[Net#a];
-  assert {:msg "  Channel invariant might not hold on action entry (generated #3)"} 0 <= R[Net#b];
-  assert {:msg "  Channel invariant might not hold on action entry (generated #4)"} 0 <= C[Net#b];
-  assert {:msg "  Channel invariant might not hold on action entry (generated #5)"} (R[Net#b] + C[Net#b]) == C#init[Net#b];
-  assert {:msg "  Channel invariant might not hold on action entry (generated #6)"} 0 <= R[Net#c];
-  assert {:msg "  Channel invariant might not hold on action entry (generated #7)"} 0 <= C[Net#c];
-  assert {:msg "  Channel invariant might not hold on action entry (generated #8)"} R[Net#c] == 0;
-  assert {:msg "  Channel invariant might not hold on action entry (generated #9)"} R[Net#a] == (R[Net#c] + C[Net#c]);
-  assert {:msg "  Channel invariant might not hold on action entry (generated #10)"} R[Net#b] == (R[Net#c] + C[Net#c]);
-  assert {:msg "  Channel invariant might not hold on action entry (generated #11)"} (forall idx$: int :: 
+  assume C[Net#c] == 0;
+  assume 0 <= R[Net#a];
+  assume 0 <= C[Net#a];
+  assume (R[Net#a] + C[Net#a]) <= L[Net#a];
+  assume 0 <= R[Net#b];
+  assume 0 <= C[Net#b];
+  assume (R[Net#b] + C[Net#b]) <= L[Net#b];
+  assume 0 <= R[Net#c];
+  assume 0 <= C[Net#c];
+  assume R[Net#c] == 0;
+  assert {:msg "  Channel invariant might not hold on action entry (#9)"} R[Net#a] == (R[Net#c] + C[Net#c]);
+  assert {:msg "  Channel invariant might not hold on action entry (#10)"} R[Net#b] == (R[Net#c] + C[Net#c]);
+  assert {:msg "  Channel invariant might not hold on action entry (#11)"} (forall idx$: int :: 
     (0 <= idx$) && (idx$ < (R[Net#c] + C[Net#c])) ==> (M[Net#c][idx$] == (M[Net#a][idx$] + M[Net#b][idx$]))
   );
 }
 procedure Net#anon$1#Add#anon$0#3()
   modifies C, R, M, St;
 {
+  var ActionPH#y: int;
   var St#next: State;
   var in1#i: int;
   var in2#j: int;
-  assume C#init[Net#a] == 1;
-  assume C#init[Net#b] == 1;
-  assume C#init[Net#c] == 0;
+  assume L[Net#a] == (1 * Base#L);
+  assume L[Net#b] == (1 * Base#L);
   assume 0 <= R[Net#a];
   assume 0 <= C[Net#a];
-  assume (R[Net#a] + C[Net#a]) == C#init[Net#a];
+  assume (R[Net#a] + C[Net#a]) <= L[Net#a];
   assume 0 <= R[Net#b];
   assume 0 <= C[Net#b];
-  assume (R[Net#b] + C[Net#b]) == C#init[Net#b];
+  assume (R[Net#b] + C[Net#b]) <= L[Net#b];
   assume 0 <= R[Net#c];
   assume 0 <= C[Net#c];
   assume R[Net#c] == 0;
@@ -103,18 +108,18 @@ procedure Net#anon$1#Add#anon$0#3()
   C[Net#b] := C[Net#b] - 1;
   M[Net#c][R[Net#c] + C[Net#c]] := in1#i + in2#j;
   C[Net#c] := C[Net#c] + 1;
-  assert {:msg "  Sub-actor action at 3.3 might not preserve the channel invariant (generated #12)"} 0 <= R[Net#a];
-  assert {:msg "  Sub-actor action at 3.3 might not preserve the channel invariant (generated #13)"} 0 <= C[Net#a];
-  assert {:msg "  Sub-actor action at 3.3 might not preserve the channel invariant (generated #14)"} (R[Net#a] + C[Net#a]) == C#init[Net#a];
-  assert {:msg "  Sub-actor action at 3.3 might not preserve the channel invariant (generated #15)"} 0 <= R[Net#b];
-  assert {:msg "  Sub-actor action at 3.3 might not preserve the channel invariant (generated #16)"} 0 <= C[Net#b];
-  assert {:msg "  Sub-actor action at 3.3 might not preserve the channel invariant (generated #17)"} (R[Net#b] + C[Net#b]) == C#init[Net#b];
-  assert {:msg "  Sub-actor action at 3.3 might not preserve the channel invariant (generated #18)"} 0 <= R[Net#c];
-  assert {:msg "  Sub-actor action at 3.3 might not preserve the channel invariant (generated #19)"} 0 <= C[Net#c];
-  assert {:msg "  Sub-actor action at 3.3 might not preserve the channel invariant (generated #20)"} R[Net#c] == 0;
-  assert {:msg "  Sub-actor action at 3.3 might not preserve the channel invariant (generated #21)"} R[Net#a] == (R[Net#c] + C[Net#c]);
-  assert {:msg "  Sub-actor action at 3.3 might not preserve the channel invariant (generated #22)"} R[Net#b] == (R[Net#c] + C[Net#c]);
-  assert {:msg "  Sub-actor action at 3.3 might not preserve the channel invariant (generated #23)"} (forall idx$: int :: 
+  assume 0 <= R[Net#a];
+  assume 0 <= C[Net#a];
+  assume (R[Net#a] + C[Net#a]) <= L[Net#a];
+  assume 0 <= R[Net#b];
+  assume 0 <= C[Net#b];
+  assume (R[Net#b] + C[Net#b]) <= L[Net#b];
+  assume 0 <= R[Net#c];
+  assume 0 <= C[Net#c];
+  assume R[Net#c] == 0;
+  assert {:msg "  Action at 3.3 ('anon$0') for actor instance 'add' might not preserve the channel invariant (#21)"} R[Net#a] == (R[Net#c] + C[Net#c]);
+  assert {:msg "  Action at 3.3 ('anon$0') for actor instance 'add' might not preserve the channel invariant (#22)"} R[Net#b] == (R[Net#c] + C[Net#c]);
+  assert {:msg "  Action at 3.3 ('anon$0') for actor instance 'add' might not preserve the channel invariant (#23)"} (forall idx$: int :: 
     (0 <= idx$) && (idx$ < (R[Net#c] + C[Net#c])) ==> (M[Net#c][idx$] == (M[Net#a][idx$] + M[Net#b][idx$]))
   );
 }
@@ -122,15 +127,14 @@ procedure Net#anon$1#exit#4()
   modifies C, R, M, St;
 {
   var ActionPH#y: int;
-  assume C#init[Net#a] == 1;
-  assume C#init[Net#b] == 1;
-  assume C#init[Net#c] == 0;
+  assume L[Net#a] == (1 * Base#L);
+  assume L[Net#b] == (1 * Base#L);
   assume 0 <= R[Net#a];
   assume 0 <= C[Net#a];
-  assume (R[Net#a] + C[Net#a]) == C#init[Net#a];
+  assume (R[Net#a] + C[Net#a]) <= L[Net#a];
   assume 0 <= R[Net#b];
   assume 0 <= C[Net#b];
-  assume (R[Net#b] + C[Net#b]) == C#init[Net#b];
+  assume (R[Net#b] + C[Net#b]) <= L[Net#b];
   assume 0 <= R[Net#c];
   assume 0 <= C[Net#c];
   assume R[Net#c] == 0;
@@ -139,12 +143,14 @@ procedure Net#anon$1#exit#4()
   assume (forall idx$: int :: 
     (0 <= idx$) && (idx$ < (R[Net#c] + C[Net#c])) ==> (M[Net#c][idx$] == (M[Net#a][idx$] + M[Net#b][idx$]))
   );
+  assume !((R[Net#a] + C[Net#a]) < L[Net#a]);
+  assume !((R[Net#b] + C[Net#b]) < L[Net#b]);
   assume !((1 <= C[Net#a]) && (1 <= C[Net#b]));
-  assert {:msg "  8.3: The network might leave unread tokens on channel a"} C[Net#a] == 0;
-  assert {:msg "  8.3: The network might leave unread tokens on channel b"} C[Net#b] == 0;
-  assert {:msg "  8.3: The network might not produce the specified number of tokens on output out"} C[Net#c] == 1;
   ActionPH#y := M[Net#c][0];
   assert {:msg "  9.13: Network action postcondition might not hold"} ActionPH#y == (M[Net#a][0] + M[Net#b][0]);
   R[Net#c] := R[Net#c] + C[Net#c];
-  C[Net#c] := 0;
+  C[Net#c] := C[Net#c] - (1 * Base#L);
+  assert {:msg "  8.3: The network might leave unread tokens on channel a"} C[Net#a] == 0;
+  assert {:msg "  8.3: The network might leave unread tokens on channel b"} C[Net#b] == 0;
+  assert {:msg "  8.3: The network might not produce the specified number of tokens on output out"} C[Net#c] == 0;
 }
