tests/AddDelay.bpl
@@ -10,13 +10,16 @@ type State;
 var M: MType;
 var C: CType;
 var R: CType;
-var C#init: CType;
+var L: CType;
 var St: [Actor]State;
+const Base#L: int;
+axiom 1 <= Base#L;
 
 const unique this#: Actor;
-
 type List a = [int]a;
 var AT#intlst: List int;
+
+function AT#Min(x:int, y: int): int { if x <= y then x else y }
 
 
 // ---------------------------------------------------------------
@@ -26,19 +29,22 @@ var AT#intlst: List int;
 procedure Add#anon$0#0()
   modifies C, R, M, St;
 {
-  var IV#in1#i: int;
-  var IV#in2#j: int;
+  var IV#in1#0: int;
+  var IV#in2#0: int;
+  assume true;
   assume true;
 }
 procedure Delay#anon$1#1()
   modifies C, R, M, St;
 {
   assume true;
+  assume true;
 }
 procedure Delay#anon$2#2()
   modifies C, R, M, St;
 {
-  var IV#in#i: int;
+  var IV#in#0: int;
+  assume true;
   assume true;
 }
 procedure Net#init#3()
@@ -57,7 +63,7 @@ procedure Net#init#3()
   M[Net#b][R[Net#b] + C[Net#b]] := ActorParam#del#k;
   C[Net#b] := C[Net#b] + 1;
   C[Net#b] := C[Net#b] - 1;
-  assert {:msg "  19.13: Network initialization might not establish the network invariant"} (M[Net#b][R[Net#b]] == M[Net#c][R[Net#c] - 1]) || (M[Net#b][R[Net#b]] == 0);
+  assert {:msg "  25.13: Network initialization might not establish the network invariant"} (M[Net#b][R[Net#b]] == M[Net#c][R[Net#c] - 1]) || (M[Net#b][R[Net#b]] == 0);
 }
 const unique Net#add: Actor;
 const unique Net#del: Actor;
@@ -69,42 +75,44 @@ procedure Net#anon$3#entry#4()
   modifies C, R, M, St;
 {
   var ActionPH#y: int;
-  assume C#init[Net#a] == 1;
-  assume C#init[Net#b] == 0;
-  assume C#init[Net#c] == 0;
-  assume C#init[Net#d] == 0;
+  assume L[Net#a] == (1 * Base#L);
   assume R[Net#a] == 0;
+  assume C[Net#a] == 0;
   assume R[Net#b] == 0;
+  assume C[Net#b] == 0;
   assume R[Net#c] == 0;
+  assume C[Net#c] == 0;
   assume R[Net#d] == 0;
-  assume C#init == C;
+  assume C[Net#d] == 0;
   C[Net#b] := C[Net#b] + 1;
   assume (M[Net#b][R[Net#b]] == M[Net#c][R[Net#c] - 1]) || (M[Net#b][R[Net#b]] == 0);
-  assert {:msg "  Channel invariant might not hold on action entry (generated #0)"} 0 <= R[Net#a];
-  assert {:msg "  Channel invariant might not hold on action entry (generated #1)"} 0 <= C[Net#a];
-  assert {:msg "  Channel invariant might not hold on action entry (generated #2)"} (R[Net#a] + C[Net#a]) == C#init[Net#a];
-  assert {:msg "  Channel invariant might not hold on action entry (generated #3)"} 0 <= R[Net#b];
-  assert {:msg "  Channel invariant might not hold on action entry (generated #4)"} 0 <= C[Net#b];
-  assert {:msg "  Channel invariant might not hold on action entry (generated #5)"} 0 <= R[Net#c];
-  assert {:msg "  Channel invariant might not hold on action entry (generated #6)"} 0 <= C[Net#c];
-  assert {:msg "  Channel invariant might not hold on action entry (generated #7)"} R[Net#c] == 0;
-  assert {:msg "  Channel invariant might not hold on action entry (generated #8)"} 0 <= R[Net#d];
-  assert {:msg "  Channel invariant might not hold on action entry (generated #9)"} 0 <= C[Net#d];
-  assert {:msg "  Channel invariant might not hold on action entry (generated #10)"} R[Net#a] == (R[Net#c] + C[Net#c]);
-  assert {:msg "  Channel invariant might not hold on action entry (generated #11)"} R[Net#b] == (R[Net#c] + C[Net#c]);
-  assert {:msg "  Channel invariant might not hold on action entry (generated #12)"} R[Net#a] == (R[Net#d] + C[Net#d]);
-  assert {:msg "  Channel invariant might not hold on action entry (generated #13)"} R[Net#b] == (R[Net#d] + C[Net#d]);
-  assert {:msg "  Channel invariant might not hold on action entry (generated #14)"} R[Net#d] == ((R[Net#b] + C[Net#b]) - 1);
-  assert {:msg "  Channel invariant might not hold on action entry (generated #15)"} (forall idx$: int :: 
+  assume 0 < M[Net#a][0];
+  assume 0 <= R[Net#a];
+  assume 0 <= C[Net#a];
+  assume (R[Net#a] + C[Net#a]) <= L[Net#a];
+  assume 0 <= R[Net#b];
+  assume 0 <= C[Net#b];
+  assume 0 <= R[Net#c];
+  assume 0 <= C[Net#c];
+  assume R[Net#c] == 0;
+  assume 0 <= R[Net#d];
+  assume 0 <= C[Net#d];
+  assert {:msg "  Channel invariant might not hold on action entry (#10)"} 0 < M[Net#a][0];
+  assert {:msg "  Channel invariant might not hold on action entry (#11)"} R[Net#a] == (R[Net#c] + C[Net#c]);
+  assert {:msg "  Channel invariant might not hold on action entry (#12)"} R[Net#b] == (R[Net#c] + C[Net#c]);
+  assert {:msg "  Channel invariant might not hold on action entry (#13)"} R[Net#a] == (R[Net#d] + C[Net#d]);
+  assert {:msg "  Channel invariant might not hold on action entry (#14)"} R[Net#b] == (R[Net#d] + C[Net#d]);
+  assert {:msg "  Channel invariant might not hold on action entry (#15)"} R[Net#d] == ((R[Net#b] + C[Net#b]) - 1);
+  assert {:msg "  Channel invariant might not hold on action entry (#16)"} (forall idx$: int :: 
     (0 <= idx$) && (idx$ < (R[Net#c] + C[Net#c])) ==> (M[Net#c][idx$] == (M[Net#a][idx$] + M[Net#b][idx$]))
   );
-  assert {:msg "  Channel invariant might not hold on action entry (generated #16)"} (forall idx$: int :: 
+  assert {:msg "  Channel invariant might not hold on action entry (#17)"} (forall idx$: int :: 
     (0 <= idx$) && (idx$ < (R[Net#d] + C[Net#d])) ==> (M[Net#d][idx$] == (M[Net#a][idx$] + M[Net#b][idx$]))
   );
-  assert {:msg "  Channel invariant might not hold on action entry (generated #17)"} (forall idx$: int :: 
+  assert {:msg "  Channel invariant might not hold on action entry (#18)"} (forall idx$: int :: 
     (1 <= idx$) && (idx$ < (R[Net#b] + C[Net#b])) ==> (M[Net#b][idx$] == M[Net#d][idx$ - 1])
   );
-  assert {:msg "  21.3: Channel invariant might not hold on action entry"} (M[Net#b][0] == M[Net#c][-1]) || (M[Net#b][0] == 0);
+  assert {:msg "  27.3: Channel invariant might not hold on action entry (#19)"} (M[Net#b][0] == M[Net#c][-1]) || (M[Net#b][0] == 0);
 }
 procedure Net#anon$3#Add#anon$0#5()
   modifies C, R, M, St;
@@ -113,13 +121,10 @@ procedure Net#anon$3#Add#anon$0#5()
   var St#next: State;
   var in1#i: int;
   var in2#j: int;
-  assume C#init[Net#a] == 1;
-  assume C#init[Net#b] == 0;
-  assume C#init[Net#c] == 0;
-  assume C#init[Net#d] == 0;
+  assume L[Net#a] == (1 * Base#L);
   assume 0 <= R[Net#a];
   assume 0 <= C[Net#a];
-  assume (R[Net#a] + C[Net#a]) == C#init[Net#a];
+  assume (R[Net#a] + C[Net#a]) <= L[Net#a];
   assume 0 <= R[Net#b];
   assume 0 <= C[Net#b];
   assume 0 <= R[Net#c];
@@ -127,6 +132,7 @@ procedure Net#anon$3#Add#anon$0#5()
   assume R[Net#c] == 0;
   assume 0 <= R[Net#d];
   assume 0 <= C[Net#d];
+  assume 0 < M[Net#a][0];
   assume R[Net#a] == (R[Net#c] + C[Net#c]);
   assume R[Net#b] == (R[Net#c] + C[Net#c]);
   assume R[Net#a] == (R[Net#d] + C[Net#d]);
@@ -154,31 +160,32 @@ procedure Net#anon$3#Add#anon$0#5()
   C[Net#c] := C[Net#c] + 1;
   M[Net#d][R[Net#d] + C[Net#d]] := in1#i + in2#j;
   C[Net#d] := C[Net#d] + 1;
-  assert {:msg "  Sub-actor action at 3.3 might not preserve the channel invariant (generated #18)"} 0 <= R[Net#a];
-  assert {:msg "  Sub-actor action at 3.3 might not preserve the channel invariant (generated #19)"} 0 <= C[Net#a];
-  assert {:msg "  Sub-actor action at 3.3 might not preserve the channel invariant (generated #20)"} (R[Net#a] + C[Net#a]) == C#init[Net#a];
-  assert {:msg "  Sub-actor action at 3.3 might not preserve the channel invariant (generated #21)"} 0 <= R[Net#b];
-  assert {:msg "  Sub-actor action at 3.3 might not preserve the channel invariant (generated #22)"} 0 <= C[Net#b];
-  assert {:msg "  Sub-actor action at 3.3 might not preserve the channel invariant (generated #23)"} 0 <= R[Net#c];
-  assert {:msg "  Sub-actor action at 3.3 might not preserve the channel invariant (generated #24)"} 0 <= C[Net#c];
-  assert {:msg "  Sub-actor action at 3.3 might not preserve the channel invariant (generated #25)"} R[Net#c] == 0;
-  assert {:msg "  Sub-actor action at 3.3 might not preserve the channel invariant (generated #26)"} 0 <= R[Net#d];
-  assert {:msg "  Sub-actor action at 3.3 might not preserve the channel invariant (generated #27)"} 0 <= C[Net#d];
-  assert {:msg "  Sub-actor action at 3.3 might not preserve the channel invariant (generated #28)"} R[Net#a] == (R[Net#c] + C[Net#c]);
-  assert {:msg "  Sub-actor action at 3.3 might not preserve the channel invariant (generated #29)"} R[Net#b] == (R[Net#c] + C[Net#c]);
-  assert {:msg "  Sub-actor action at 3.3 might not preserve the channel invariant (generated #30)"} R[Net#a] == (R[Net#d] + C[Net#d]);
-  assert {:msg "  Sub-actor action at 3.3 might not preserve the channel invariant (generated #31)"} R[Net#b] == (R[Net#d] + C[Net#d]);
-  assert {:msg "  Sub-actor action at 3.3 might not preserve the channel invariant (generated #32)"} R[Net#d] == ((R[Net#b] + C[Net#b]) - 1);
-  assert {:msg "  Sub-actor action at 3.3 might not preserve the channel invariant (generated #33)"} (forall idx$: int :: 
+  assume 0 <= R[Net#a];
+  assume 0 <= C[Net#a];
+  assume (R[Net#a] + C[Net#a]) <= L[Net#a];
+  assume 0 <= R[Net#b];
+  assume 0 <= C[Net#b];
+  assume 0 <= R[Net#c];
+  assume 0 <= C[Net#c];
+  assume R[Net#c] == 0;
+  assume 0 <= R[Net#d];
+  assume 0 <= C[Net#d];
+  assert {:msg "  Action at 3.3 ('anon$0') for actor instance 'add' might not preserve the channel invariant (#30)"} 0 < M[Net#a][0];
+  assert {:msg "  Action at 3.3 ('anon$0') for actor instance 'add' might not preserve the channel invariant (#31)"} R[Net#a] == (R[Net#c] + C[Net#c]);
+  assert {:msg "  Action at 3.3 ('anon$0') for actor instance 'add' might not preserve the channel invariant (#32)"} R[Net#b] == (R[Net#c] + C[Net#c]);
+  assert {:msg "  Action at 3.3 ('anon$0') for actor instance 'add' might not preserve the channel invariant (#33)"} R[Net#a] == (R[Net#d] + C[Net#d]);
+  assert {:msg "  Action at 3.3 ('anon$0') for actor instance 'add' might not preserve the channel invariant (#34)"} R[Net#b] == (R[Net#d] + C[Net#d]);
+  assert {:msg "  Action at 3.3 ('anon$0') for actor instance 'add' might not preserve the channel invariant (#35)"} R[Net#d] == ((R[Net#b] + C[Net#b]) - 1);
+  assert {:msg "  Action at 3.3 ('anon$0') for actor instance 'add' might not preserve the channel invariant (#36)"} (forall idx$: int :: 
     (0 <= idx$) && (idx$ < (R[Net#c] + C[Net#c])) ==> (M[Net#c][idx$] == (M[Net#a][idx$] + M[Net#b][idx$]))
   );
-  assert {:msg "  Sub-actor action at 3.3 might not preserve the channel invariant (generated #34)"} (forall idx$: int :: 
+  assert {:msg "  Action at 3.3 ('anon$0') for actor instance 'add' might not preserve the channel invariant (#37)"} (forall idx$: int :: 
     (0 <= idx$) && (idx$ < (R[Net#d] + C[Net#d])) ==> (M[Net#d][idx$] == (M[Net#a][idx$] + M[Net#b][idx$]))
   );
-  assert {:msg "  Sub-actor action at 3.3 might not preserve the channel invariant (generated #35)"} (forall idx$: int :: 
+  assert {:msg "  Action at 3.3 ('anon$0') for actor instance 'add' might not preserve the channel invariant (#38)"} (forall idx$: int :: 
     (1 <= idx$) && (idx$ < (R[Net#b] + C[Net#b])) ==> (M[Net#b][idx$] == M[Net#d][idx$ - 1])
   );
-  assert {:msg "  21.3: Sub-actor action at 3.3 might not preserve the channel invariant"} (M[Net#b][0] == M[Net#c][-1]) || (M[Net#b][0] == 0);
+  assert {:msg "  27.3: Action at 3.3 ('anon$0') for actor instance 'add' might not preserve the channel invariant (#39)"} (M[Net#b][0] == M[Net#c][-1]) || (M[Net#b][0] == 0);
 }
 procedure Net#anon$3#Delay#anon$2#6()
   modifies C, R, M, St;
@@ -188,13 +195,10 @@ procedure Net#anon$3#Delay#anon$2#6()
   var St#next: State;
   var in#i: int;
   assume ActorParam#k == 0;
-  assume C#init[Net#a] == 1;
-  assume C#init[Net#b] == 0;
-  assume C#init[Net#c] == 0;
-  assume C#init[Net#d] == 0;
+  assume L[Net#a] == (1 * Base#L);
   assume 0 <= R[Net#a];
   assume 0 <= C[Net#a];
-  assume (R[Net#a] + C[Net#a]) == C#init[Net#a];
+  assume (R[Net#a] + C[Net#a]) <= L[Net#a];
   assume 0 <= R[Net#b];
   assume 0 <= C[Net#b];
   assume 0 <= R[Net#c];
@@ -202,6 +206,7 @@ procedure Net#anon$3#Delay#anon$2#6()
   assume R[Net#c] == 0;
   assume 0 <= R[Net#d];
   assume 0 <= C[Net#d];
+  assume 0 < M[Net#a][0];
   assume R[Net#a] == (R[Net#c] + C[Net#c]);
   assume R[Net#b] == (R[Net#c] + C[Net#c]);
   assume R[Net#a] == (R[Net#d] + C[Net#d]);
@@ -224,43 +229,9 @@ procedure Net#anon$3#Delay#anon$2#6()
   C[Net#d] := C[Net#d] - 1;
   M[Net#b][R[Net#b] + C[Net#b]] := in#i;
   C[Net#b] := C[Net#b] + 1;
-  assert {:msg "  Sub-actor action at 9.3 might not preserve the channel invariant (generated #36)"} 0 <= R[Net#a];
-  assert {:msg "  Sub-actor action at 9.3 might not preserve the channel invariant (generated #37)"} 0 <= C[Net#a];
-  assert {:msg "  Sub-actor action at 9.3 might not preserve the channel invariant (generated #38)"} (R[Net#a] + C[Net#a]) == C#init[Net#a];
-  assert {:msg "  Sub-actor action at 9.3 might not preserve the channel invariant (generated #39)"} 0 <= R[Net#b];
-  assert {:msg "  Sub-actor action at 9.3 might not preserve the channel invariant (generated #40)"} 0 <= C[Net#b];
-  assert {:msg "  Sub-actor action at 9.3 might not preserve the channel invariant (generated #41)"} 0 <= R[Net#c];
-  assert {:msg "  Sub-actor action at 9.3 might not preserve the channel invariant (generated #42)"} 0 <= C[Net#c];
-  assert {:msg "  Sub-actor action at 9.3 might not preserve the channel invariant (generated #43)"} R[Net#c] == 0;
-  assert {:msg "  Sub-actor action at 9.3 might not preserve the channel invariant (generated #44)"} 0 <= R[Net#d];
-  assert {:msg "  Sub-actor action at 9.3 might not preserve the channel invariant (generated #45)"} 0 <= C[Net#d];
-  assert {:msg "  Sub-actor action at 9.3 might not preserve the channel invariant (generated #46)"} R[Net#a] == (R[Net#c] + C[Net#c]);
-  assert {:msg "  Sub-actor action at 9.3 might not preserve the channel invariant (generated #47)"} R[Net#b] == (R[Net#c] + C[Net#c]);
-  assert {:msg "  Sub-actor action at 9.3 might not preserve the channel invariant (generated #48)"} R[Net#a] == (R[Net#d] + C[Net#d]);
-  assert {:msg "  Sub-actor action at 9.3 might not preserve the channel invariant (generated #49)"} R[Net#b] == (R[Net#d] + C[Net#d]);
-  assert {:msg "  Sub-actor action at 9.3 might not preserve the channel invariant (generated #50)"} R[Net#d] == ((R[Net#b] + C[Net#b]) - 1);
-  assert {:msg "  Sub-actor action at 9.3 might not preserve the channel invariant (generated #51)"} (forall idx$: int :: 
-    (0 <= idx$) && (idx$ < (R[Net#c] + C[Net#c])) ==> (M[Net#c][idx$] == (M[Net#a][idx$] + M[Net#b][idx$]))
-  );
-  assert {:msg "  Sub-actor action at 9.3 might not preserve the channel invariant (generated #52)"} (forall idx$: int :: 
-    (0 <= idx$) && (idx$ < (R[Net#d] + C[Net#d])) ==> (M[Net#d][idx$] == (M[Net#a][idx$] + M[Net#b][idx$]))
-  );
-  assert {:msg "  Sub-actor action at 9.3 might not preserve the channel invariant (generated #53)"} (forall idx$: int :: 
-    (1 <= idx$) && (idx$ < (R[Net#b] + C[Net#b])) ==> (M[Net#b][idx$] == M[Net#d][idx$ - 1])
-  );
-  assert {:msg "  21.3: Sub-actor action at 9.3 might not preserve the channel invariant"} (M[Net#b][0] == M[Net#c][-1]) || (M[Net#b][0] == 0);
-}
-procedure Net#anon$3#exit#7()
-  modifies C, R, M, St;
-{
-  var ActionPH#y: int;
-  assume C#init[Net#a] == 1;
-  assume C#init[Net#b] == 0;
-  assume C#init[Net#c] == 0;
-  assume C#init[Net#d] == 0;
   assume 0 <= R[Net#a];
   assume 0 <= C[Net#a];
-  assume (R[Net#a] + C[Net#a]) == C#init[Net#a];
+  assume (R[Net#a] + C[Net#a]) <= L[Net#a];
   assume 0 <= R[Net#b];
   assume 0 <= C[Net#b];
   assume 0 <= R[Net#c];
@@ -268,6 +239,39 @@ procedure Net#anon$3#exit#7()
   assume R[Net#c] == 0;
   assume 0 <= R[Net#d];
   assume 0 <= C[Net#d];
+  assert {:msg "  Action at 9.3 ('anon$2') for actor instance 'del' might not preserve the channel invariant (#50)"} 0 < M[Net#a][0];
+  assert {:msg "  Action at 9.3 ('anon$2') for actor instance 'del' might not preserve the channel invariant (#51)"} R[Net#a] == (R[Net#c] + C[Net#c]);
+  assert {:msg "  Action at 9.3 ('anon$2') for actor instance 'del' might not preserve the channel invariant (#52)"} R[Net#b] == (R[Net#c] + C[Net#c]);
+  assert {:msg "  Action at 9.3 ('anon$2') for actor instance 'del' might not preserve the channel invariant (#53)"} R[Net#a] == (R[Net#d] + C[Net#d]);
+  assert {:msg "  Action at 9.3 ('anon$2') for actor instance 'del' might not preserve the channel invariant (#54)"} R[Net#b] == (R[Net#d] + C[Net#d]);
+  assert {:msg "  Action at 9.3 ('anon$2') for actor instance 'del' might not preserve the channel invariant (#55)"} R[Net#d] == ((R[Net#b] + C[Net#b]) - 1);
+  assert {:msg "  Action at 9.3 ('anon$2') for actor instance 'del' might not preserve the channel invariant (#56)"} (forall idx$: int :: 
+    (0 <= idx$) && (idx$ < (R[Net#c] + C[Net#c])) ==> (M[Net#c][idx$] == (M[Net#a][idx$] + M[Net#b][idx$]))
+  );
+  assert {:msg "  Action at 9.3 ('anon$2') for actor instance 'del' might not preserve the channel invariant (#57)"} (forall idx$: int :: 
+    (0 <= idx$) && (idx$ < (R[Net#d] + C[Net#d])) ==> (M[Net#d][idx$] == (M[Net#a][idx$] + M[Net#b][idx$]))
+  );
+  assert {:msg "  Action at 9.3 ('anon$2') for actor instance 'del' might not preserve the channel invariant (#58)"} (forall idx$: int :: 
+    (1 <= idx$) && (idx$ < (R[Net#b] + C[Net#b])) ==> (M[Net#b][idx$] == M[Net#d][idx$ - 1])
+  );
+  assert {:msg "  27.3: Action at 9.3 ('anon$2') for actor instance 'del' might not preserve the channel invariant (#59)"} (M[Net#b][0] == M[Net#c][-1]) || (M[Net#b][0] == 0);
+}
+procedure Net#anon$3#exit#7()
+  modifies C, R, M, St;
+{
+  var ActionPH#y: int;
+  assume L[Net#a] == (1 * Base#L);
+  assume 0 <= R[Net#a];
+  assume 0 <= C[Net#a];
+  assume (R[Net#a] + C[Net#a]) <= L[Net#a];
+  assume 0 <= R[Net#b];
+  assume 0 <= C[Net#b];
+  assume 0 <= R[Net#c];
+  assume 0 <= C[Net#c];
+  assume R[Net#c] == 0;
+  assume 0 <= R[Net#d];
+  assume 0 <= C[Net#d];
+  assume 0 < M[Net#a][0];
   assume R[Net#a] == (R[Net#c] + C[Net#c]);
   assume R[Net#b] == (R[Net#c] + C[Net#c]);
   assume R[Net#a] == (R[Net#d] + C[Net#d]);
@@ -283,15 +287,17 @@ procedure Net#anon$3#exit#7()
     (1 <= idx$) && (idx$ < (R[Net#b] + C[Net#b])) ==> (M[Net#b][idx$] == M[Net#d][idx$ - 1])
   );
   assume (M[Net#b][0] == M[Net#c][-1]) || (M[Net#b][0] == 0);
-  assume !(((1 <= C[Net#a]) && (1 <= C[Net#b])) || (1 <= C[Net#d]));
+  assume !((R[Net#a] + C[Net#a]) < L[Net#a]);
+  assume !((1 <= C[Net#a]) && (1 <= C[Net#b]));
+  assume !(1 <= C[Net#d]);
   ActionPH#y := M[Net#c][0];
-  assert {:msg "  15.13: Network action postcondition might not hold"} (ActionPH#y == (M[Net#c][R[Net#c] - 1] + M[Net#a][0])) || (ActionPH#y == M[Net#a][0]);
+  assert {:msg "  21.13: Network action postcondition might not hold"} (ActionPH#y == (M[Net#c][R[Net#c] - 1] + M[Net#a][0])) || (ActionPH#y == M[Net#a][0]);
   R[Net#c] := R[Net#c] + C[Net#c];
-  C[Net#c] := C[Net#c] - 1;
+  C[Net#c] := C[Net#c] - (1 * Base#L);
   C[Net#b] := C[Net#b] - 1;
-  assert {:msg "  19.13: The network might not preserve the network invariant"} (M[Net#b][R[Net#b]] == M[Net#c][R[Net#c] - 1]) || (M[Net#b][R[Net#b]] == 0);
-  assert {:msg "  14.3: The network might leave unread tokens on channel a"} C[Net#a] == 0;
-  assert {:msg "  14.3: The network might leave unread tokens on channel b"} C[Net#b] == 0;
-  assert {:msg "  14.3: The network might not produce the specified number of tokens on output out"} C[Net#c] == 0;
-  assert {:msg "  14.3: The network might leave unread tokens on channel d"} C[Net#d] == 0;
+  assert {:msg "  25.13: The network might not preserve the network invariant"} (M[Net#b][R[Net#b]] == M[Net#c][R[Net#c] - 1]) || (M[Net#b][R[Net#b]] == 0);
+  assert {:msg "  19.3: The network might leave unread tokens on channel a"} C[Net#a] == 0;
+  assert {:msg "  19.3: The network might leave unread tokens on channel b"} C[Net#b] == 0;
+  assert {:msg "  19.3: The network might not produce the specified number of tokens on output out"} C[Net#c] == 0;
+  assert {:msg "  19.3: The network might leave unread tokens on channel d"} C[Net#d] == 0;
 }
